More multiset groundwork

TermRewriting/MultisetOrders_2_5.lean
@@ -4,19 +4,58 @@ variable (R S : α → α → Prop)
 
 def MultisetOver α := α → Nat
 
-def MultisetOver.Finite (m : MultisetOver α) := Set.Finite { x | m x > 0 }
+def MultisetOver.Mem (x : α) (m : MultisetOver α) := m x > 0
+
+def MultisetOver.Finite (m : MultisetOver α) := Set.Finite { x | Mem x m }
+
+def MultisetOver.Nonempty (m : MultisetOver α) := Set.Nonempty { x | Mem x m }
 
 def FinMultisetOver α := { m : MultisetOver α // MultisetOver.Finite m }
 
-def MultisetOver.Mem (x : α) (m : MultisetOver α) := m x > 0
+@[simp]
 def MultisetOver.Subset (m₁ m₂ : MultisetOver α) := ∀x, m₁ x ≤ m₂ x
+
+@[simp]
 def MultisetOver.Union (m₁ m₂ : MultisetOver α) := λx ↦ m₁ x + m₂ x
+
+@[simp]
 def MultisetOver.Difference (m₁ m₂ : MultisetOver α) := λx ↦ m₁ x - m₂ x
 def MultisetOver.Empty := λ_ : α ↦ 0
 
 def MultisetOver.ordering (m₁ m₂ : MultisetOver α) := 
   ∃X Y : FinMultisetOver α,
-    (X.1 ≠ MultisetOver.Empty) ∧
-    (MultisetOver.Subset X.1 m₁) ∧
-    (m₂ = MultisetOver.Union (MultisetOver.Difference m₁ X.1) Y.1) ∧
+    Nonempty X.1 ∧
+    MultisetOver.Subset X.1 m₁ ∧
+    m₂ = MultisetOver.Union (MultisetOver.Difference m₁ X.1) Y.1 ∧
     ∀y, MultisetOver.Mem y Y.1 → ∃x, MultisetOver.Mem x X.1 ∧ R x y
+
+theorem MultisetOver.ofStrictOrder : isStrictOrder R → isStrictOrder (ordering R) := by
+  intro strict; constructor
+  case irref =>
+    rintro x ⟨X,Y,inhab,sub,eq,cond⟩
+    have : X = Y := by
+      apply Subtype.eq
+      funext el
+      have : x el + X.val el = X.val el + (x el - X.val el) +  Y.val el  := by
+        conv => lhs; rw [eq]
+        simp_arith
+      rw [Nat.add_sub_cancel' (sub el)] at this 
+      simp_arith at this
+      assumption
+    rw [this] at cond
+    rw [this] at inhab
+    have : ∀x : { z | Mem z Y.val }, ∃y : { z | Mem z Y.val}, R y x := by 
+      intro x; have ⟨y, yprop⟩ := cond x.val x.prop; exists ⟨y, yprop.1⟩; simp; exact yprop.2
+    unfold Nonempty at inhab; unfold Set.Nonempty at inhab
+    have ⟨a,prop⟩ := inhab
+    have ⟨chain,cprop⟩ := descending.fromAE (λ x y : { z | Mem z Y.val} ↦ R y x) ⟨a,prop⟩ this
+    have strict_conv := (StrictOrder.of_converse R).mpr strict
+    sorry
+  all_goals sorry
+
+
+
+    --apply Set.Finite.not_infinite X.prop
+
+
+
